Sorry free

src/cnf.lean
@@ -20,13 +20,36 @@ end
 
 namespace literal
 
+@[simp]
 def inverse : literal α → literal α
 | (pos x) := neg x
 | (neg x) := pos x
 
+@[simp]
+def var : literal α → α
+| (pos x) := x
+| (neg x) := x
+
+@[simp]
 def satisfied (ι : interpretation α) : literal α → bool
 | (pos x) := ι x
 | (neg x) := bnot (ι x)
+
+@[simp]
+lemma satisfied_inverse (ι : interpretation α) (l : literal α) : satisfied ι l.inverse = bnot (satisfied ι l) :=
+by cases l; simp
+
+@[simp]
+lemma inverse_inverse (l : literal α) : l.inverse.inverse = l :=
+by cases l; refl
+
+@[simp]
+lemma bnot_iff_not (b : bool) : !b ↔ ¬b :=
+by { unfold_coes, simp only [bnot_eq_true_eq_eq_ff, eq_ff_eq_not_eq_tt] }
+
+lemma not_satisfied_and_satisfied_inverse (ι : interpretation α) (l m : literal α)
+  (hl : satisfied ι l) (hm : satisfied ι m) : l ≠ m.inverse :=
+λ h, absurd hl $ by { convert hm, simp [h] }
 
 end literal
 
@@ -35,9 +58,24 @@ namespace clause
 def satisfied (ι : interpretation α) (c : clause α) : bool :=
 c.any (literal.satisfied ι)
 
+lemma satisfied_eq {ι κ : interpretation α} {c : clause α} (h : ∀ l ∈ c, literal.satisfied ι l = literal.satisfied κ l) :
+  c.satisfied ι = c.satisfied κ :=
+begin
+  induction c with l ls ih,
+  { refl },
+  { rw [satisfied, satisfied, list.any_cons, list.any_cons, h l (list.mem_cons_self _ _), ←satisfied, ←satisfied,
+      ih (λ m hm, h _ (list.mem_cons_of_mem _ hm))] }
+end
+
+lemma satisfied_iff (ι : interpretation α) (c : clause α) : satisfied ι c ↔ ∃ l ∈ c, literal.satisfied ι l :=
+by rw [satisfied, list.any_iff_exists]
+
 @[simp] 
 lemma not_satisfied_empty (ι : interpretation α) : satisfied ι [] = ff :=
 rfl
+
+lemma not_satisfied_empty' (ι : interpretation α) : ¬satisfied ι [] :=
+by simp
 
 end clause
 
@@ -46,10 +84,43 @@ namespace cnf
 def satisfied (ι : interpretation α) (c : cnf α) : bool :=
 c.all (clause.satisfied ι)
 
+lemma satisfied_eq (ι κ : interpretation α) {c : cnf α} (h : ∀ γ ∈ c, ∀ l ∈ γ, literal.satisfied ι l = literal.satisfied κ l) :
+  c.satisfied ι = c.satisfied κ :=
+begin
+  induction c with γ c ih,
+  { refl },
+  { rw [satisfied, satisfied, list.all_cons, list.all_cons,
+      clause.satisfied_eq (λ l hl, h _ (list.mem_cons_self _ _) _ hl), ←satisfied, ←satisfied,
+      ih (λ δ hδ l hl, h _ (list.mem_cons_of_mem _ hδ) _ hl)] }
+end
+
+lemma satisfied_iff (ι : interpretation α) (c : cnf α) : satisfied ι c ↔ ∀ γ ∈ c, clause.satisfied ι γ :=
+by rw [satisfied, list.all_iff_forall]
+
 def satisfiable (c : cnf α) : Prop :=
 ∃ ι, satisfied ι c
 
+@[simp]
 lemma satisfiable_empty : satisfiable ([] : cnf α) :=
 ⟨λ x, false, dec_trivial⟩
+
+lemma not_satisfiable_of_empty_mem {c : cnf α} (hc : [] ∈ c) : ¬satisfiable c :=
+begin
+  rw satisfiable,
+  rintro ⟨ι, hι⟩,
+  rw satisfied_iff at hι,
+  exact clause.not_satisfied_empty' ι (hι _ hc)
+end
+
+#print axioms not_satisfiable_of_empty_mem
+
+def size (c : cnf α) : ℕ :=
+(c.map list.length).sum
+
+instance : has_sizeof (cnf α) :=
+{ sizeof := size }
+
+lemma sizeof_eq_size (c : cnf α) : sizeof c = size c :=
+rfl
 
 end cnf
